examples/list_queries.v
@@ -10,6 +10,8 @@ Load list.
 Goal forall (xs rs : list nat), rev xs rs -> xs = rs.
 intros xs rs H.
 elpi dep_pbt 3 (H) (xs).
+elpi dep_pbt size 10 (H) (xs).
+elpi dep_pbt pair 3 7 (H) (xs).
 Abort.
 
 (* same query, different type*)
@@ -27,7 +29,7 @@ Abort.
 (* This property is true *)
 Goal forall (xs rs : list nat), rev xs rs -> rev rs xs.
 intros xs rs  H.
-Fail elpi dep_pbt 3 (H) (xs).
+Fail elpi dep_pbt 2 (H) (xs).
 Abort.
 
 (* true *)
@@ -41,7 +43,7 @@ Goal forall (xs ys aps raps rxs rys : list nat),
 append xs ys aps -> rev xs rxs -> rev ys rys ->
 rev aps raps -> append rxs rys raps.
 intros.
-elpi dep_pbt 5 (H /\ H0 /\ H1 /\ H2 ) (xs) (ys).
+elpi dep_pbt 3 (H /\ H0 /\ H1 /\ H2 ) (xs) (ys).
 Abort.
 
 Goal forall x x' y: list nat,
@@ -50,8 +52,3 @@ intros.
 elpi dep_pbt 3 (H /\ H0) (x).
 Abort.
 
-(*Goal forall x y: list nat,
-rev (app [2] x) y.
-
-intros.
-elpi dep_pbt 3 (True) (x).*)
